src/MinLTL.v
@@ -1,5 +1,7 @@
 Require Import
+  Coq.Classes.Equivalence
   Coq.Classes.Morphisms
+  Coq.Classes.SetoidClass
   Bool.
 
 (***********************************************************************
@@ -20,11 +22,31 @@ Include Bool.
 Parameter next : t -> t.
 Parameter until : t -> t -> t.
 
-Declare Instance next_equiv : Proper (equiv ==> equiv) next.
-Declare Instance until_equiv : Proper (equiv ==> equiv ==> equiv) until.
+Declare Instance next_respects_impl :
+  Proper (impl ==> impl) next.
+Declare Instance until_respects_impl :
+  Proper (impl ==> impl ==> impl) until.
 
-Notation "◯ p"     := (next p)    (at level 0).
-Notation "p 'U' q" := (until p q) (at level 45).
+Program Instance next_respects_eqv :
+  Proper (eqv ==> eqv) next.
+Next Obligation.
+  repeat intro.
+  destruct H; split.
+  - now rewrite H.
+  - now rewrite H0.
+Qed.
+
+Program Instance until_respects_eqv :
+  Proper (eqv ==> eqv ==> eqv) until.
+Next Obligation.
+  repeat intro.
+  destruct H, H0; split.
+  - now rewrite H, H0.
+  - now rewrite H1, H2.
+Qed.
+
+Notation "◯ p"     := (next p)    (at level 0, right associativity).
+Notation "p 'U' q" := (until p q) (at level 45, right associativity).
 
 (*** 3.1 Next *)
 
@@ -57,16 +79,9 @@ Qed.
 
 Lemma (* 6 *) next_distr_next_eq (φ ψ : t) : ◯ (φ ≡ ψ) ≈ ◯ φ ≡ ◯ ψ.
 Proof.
-  rewrite next_distr_or.
-  rewrite not_or.
-  rewrite next_distr_and.
-  rewrite next_self_dual.
-  rewrite next_self_dual.
-  rewrite not_and.
-  rewrite next_distr_or.
-  rewrite next_self_dual.
-  rewrite <- not_and.
-  now rewrite <- not_or.
+  rewrite !next_distr_or.
+  rewrite !next_self_dual.
+  now rewrite next_distr_and.
 Qed.
 
 Lemma (* 7 *) next_top : ◯ (⊤) ≈ ⊤.
@@ -88,22 +103,38 @@ Qed.
 
 (*** 3.2 Until *)
 
-Hypothesis (* 9 *) next_distr_until : forall (φ ψ : t), ◯ (φ U ψ) ≈ (◯ φ) U (◯ ψ).
-Hypothesis (* 10 *) until_expansion : forall (φ ψ : t), φ U ψ ≈ ψ ∨ (φ ∧ ◯ (φ U ψ)).
-Hypothesis (* 11 *) until_right_bottom : forall (φ : t), φ U ⊥ ≈ ⊥.
-Hypothesis (* 12 *) until_left_distr_or : forall (φ ψ χ : t), φ U (ψ ∨ χ) ≈ (φ U ψ) ∨ (φ U χ).
-Hypothesis (* 13 *) until_right_distr_or : forall (φ ψ χ : t), (φ U χ) ∨ (ψ U χ) ⟹ (φ ∨ ψ) U χ.
-Hypothesis (* 14 *) until_left_distr_and : forall (φ ψ χ : t), φ U (ψ ∧ χ) ⟹ (φ U ψ) ∧ (φ U χ).
-Hypothesis (* 15 *) until_right_distr_and : forall (φ ψ χ : t), (φ ∧ ψ) U χ ≈ (φ U χ) ∧ (ψ U χ).
-Hypothesis (* 16 *) until_impl_order : forall (φ ψ χ : t), (φ U ψ) ∧ (¬ ψ U χ) ⟹ φ U χ.
-Hypothesis (* 17 *) until_right_or_order : forall (φ ψ χ : t), φ U (ψ U χ) ⟹ (φ ∨ ψ) U χ.
-Hypothesis (* 18 *) until_right_and_order : forall (φ ψ χ : t), φ U (ψ ∧ χ) ⟹ φ U (ψ U χ).
+Hypothesis (* 9 *) next_distr_until : forall (φ ψ : t),
+  ◯ (φ U ψ) ≈ (◯ φ) U (◯ ψ).
+Hypothesis (* 10 *) until_expansion : forall (φ ψ : t),
+  φ U ψ ≈ ψ ∨ (φ ∧ ◯ (φ U ψ)).
+Hypothesis (* 11 *) until_right_bottom : forall (φ : t),
+  φ U ⊥ ≈ ⊥.
+Hypothesis (* 12 *) until_left_distr_or : forall (φ ψ χ : t),
+  φ U (ψ ∨ χ) ≈ (φ U ψ) ∨ (φ U χ).
+Hypothesis (* 13 *) until_right_distr_or : forall (φ ψ χ : t),
+  (φ U χ) ∨ (ψ U χ) ⟹ (φ ∨ ψ) U χ.
+Hypothesis (* 14 *) until_left_distr_and : forall (φ ψ χ : t),
+  φ U (ψ ∧ χ) ⟹ (φ U ψ) ∧ (φ U χ).
+Hypothesis (* 15 *) until_right_distr_and : forall (φ ψ χ : t),
+  (φ ∧ ψ) U χ ≈ (φ U χ) ∧ (ψ U χ).
+Hypothesis (* 16 *) until_impl_order : forall (φ ψ χ : t),
+  (φ U ψ) ∧ (¬ ψ U χ) ⟹ φ U χ.
+Hypothesis (* 17 *) until_right_or_order : forall (φ ψ χ : t),
+  φ U (ψ U χ) ⟹ (φ ∨ ψ) U χ.
+Hypothesis (* 18 *) until_right_and_order : forall (φ ψ χ : t),
+  φ U (ψ ∧ χ) ⟹ φ U (ψ U χ).
 
-(* Lemmas 19-37 *)
-
-Lemma (* 19 *) until_right_distr_impl (φ ψ χ : t) : (φ → ψ) U χ ⟹ (φ U χ) → (ψ U χ).
+Lemma (* 19 *) until_right_distr_impl (φ ψ χ : t) :
+  (φ → ψ) U χ ⟹ (φ U χ) → (ψ U χ).
 Proof.
-Admitted.
+  apply and_impl_iff.
+  rewrite <- until_right_distr_and.
+  rewrite and_comm.
+  rewrite and_impl.
+  rewrite until_right_distr_and.
+  rewrite and_comm.
+  now apply and_proj.
+Qed.
 
 Lemma (* 20 *) until_right_top (φ : t) : φ U ⊤ ≈ ⊤.
 Proof.
@@ -138,7 +169,7 @@ Proof.
   rewrite until_right_or_order.
   rewrite until_right_distr_impl.
   rewrite and_comm.
-  rewrite distr_or_and.
+  rewrite and_distr_or.
   rewrite absurdity.
   rewrite or_comm.
   rewrite or_false.
@@ -161,7 +192,7 @@ Admitted.
 Lemma (* 28 *) until_28 (φ ψ : t) : φ U ψ ⟹ φ ∨ ψ.
 Proof.
   rewrite until_expansion.
-  rewrite distr_and_or.
+  rewrite or_distr_and.
   rewrite and_proj.
   rewrite or_comm.
   reflexivity.
@@ -183,7 +214,7 @@ Qed.
 
 Lemma (* 31 *) until_absorb_or_u (φ ψ : t) : φ ∨ (φ U ψ) ≈ φ ∨ ψ.
 Proof.
-  apply equiv_def; split.
+  split.
   - rewrite (until_28 φ ψ) at 1.
     rewrite <- or_assoc.
     now rewrite or_idem.
@@ -200,7 +231,7 @@ Qed.
 
 Lemma (* 33 *) until_absorb_u_and (φ ψ : t) : (φ U ψ) ∧ ψ ≈ ψ.
 Proof.
-  apply equiv_def; split.
+  split.
   - rewrite and_comm.
     now apply and_proj.
   - rewrite <- and_idem at 1.
@@ -209,7 +240,7 @@ Qed.
 
 Lemma (* 34 *) until_absorb_u_or_and (φ ψ : t) : (φ U ψ) ∨ (φ ∧ ψ) ≈ φ U ψ.
 Proof.
-  apply equiv_def; split.
+  split.
   - rewrite until_30.
     now rewrite or_idem.
   - now rewrite <- or_inj.
@@ -217,7 +248,7 @@ Qed.
 
 Lemma (* 35 *) until_absorb_u_and_or (φ ψ : t) : (φ U ψ) ∧ (φ ∨ ψ) ≈ φ U ψ.
 Proof.
-  apply equiv_def; split.
+  split.
   - now apply and_proj.
   - rewrite <- until_28.
     now rewrite and_idem.
@@ -225,7 +256,7 @@ Qed.
 
 Lemma (* 36 *) until_left_absorb (φ ψ : t) : φ U (φ U ψ) ≈ φ U ψ.
 Proof.
-  apply equiv_def; split.
+  split.
   - rewrite until_right_or_order.
     now rewrite or_idem.
   - now apply until_insertion.
